fiat2/src/fiat2/SumAgg.v
@@ -1,0 +1,290 @@
+Require Import fiat2.Language fiat2.Interpret fiat2.Value fiat2.TypeSystem fiat2.TypeSound fiat2.IndexInterface2 fiat2.CollectionTransf fiat2.Utils fiat2.TransfSound fiat2.TransfUtils fiat2.Substitute.
+Require Import coqutil.Map.Interface coqutil.Word.Interface coqutil.Datatypes.Result.
+Require Import List String ZArith Permutation Sorted.
+Import ListNotations.
+
+Open Scope string_scope.
+
+
+Section WithHole.
+  Context (hole : string).
+  Context (attr : string).
+
+  Section WithVars.
+    Context (tup acc x : string).
+    Context (H_NoDup : is_NoDup_opaque [tup; acc; x]).
+
+    Definition to_idx : expr :=
+      EACFold AGSum (EProj LikeBag (EBagOf (EVar hole)) x (EAccess (EVar x) attr)).
+
+    Definition is_tbl_ty (t : type) : bool :=
+      match t with
+      | TList (TRecord rt) => match access_record rt attr with
+                              | Success t => type_eqb t TInt
+                              | _ => false
+                              end
+      | _ => false
+      end.
+
+    Definition idx_ty (t : type) : type := TInt.
+
+    Lemma idx_ty_wf : forall t, type_wf t -> is_tbl_ty t = true -> type_wf (idx_ty t).
+      intros; constructor.
+    Qed.
+
+    Section WithMap.
+      Context {tenv : map.map string type} {tenv_ok : map.ok tenv}.
+      Context {width: Z} {word: word.word width} {word_ok: word.ok word}.
+      Notation value := (value (width:=width)).
+      Context {locals : map.map string value} {locals_ok : map.ok locals}.
+
+      Definition idx_wf (tbl_v agg_v : value) : Prop :=
+        agg_v = interp_expr map.empty (map.put map.empty hole tbl_v) to_idx.
+
+      Lemma to_idx_ty : forall (t : type),
+          type_wf t -> is_tbl_ty t = true ->
+          type_of map.empty (map.put map.empty hole t) to_idx (idx_ty t).
+      Proof.
+        unfold is_tbl_ty, to_idx, idx_ty; intros.
+        repeat destruct_match_hyp; try discriminate.
+        rewrite type_eqb_eq in *; subst.
+        repeat econstructor; repeat rewrite_map_get_put_goal; eauto.
+      Qed.
+
+      Lemma to_idx_wf : forall (v : value) (t : type),
+          type_wf t -> is_tbl_ty t = true ->
+          type_of_value v t ->
+          idx_wf v (interp_expr map.empty (map.put map.empty hole v) to_idx).
+      Proof.
+        unfold idx_wf; intros; auto.
+      Qed.
+
+
+      Instance sum_agg : IndexInterface2.index := IndexInterface2.mk hole to_idx idx_ty is_tbl_ty.
+
+      Instance sum_agg_ok : IndexInterface2.ok sum_agg idx_wf :=
+        IndexInterface2.Build_ok sum_agg idx_wf idx_ty_wf to_idx_ty to_idx_wf.
+
+      (* ??? move to utils *)
+      Lemma Forall2_access_record : forall A A' P l l' x (a : A) (a' : A'),
+          Forall2 (fun p p' => fst p = fst p' /\ P (snd p) (snd p')) l l' ->
+          access_record l x = Success a ->
+          access_record l' x = Success a' ->
+          P a a'.
+      Proof.
+        induction 1; cbn; try discriminate; auto.
+        repeat case_match; cbn in *; intuition idtac;
+          repeat (try clear_refl; do_injection); subst; auto;
+          congruence.
+      Qed.
+
+      Ltac invert_type_of_aggr_clear :=
+        lazymatch goal with
+        | H: type_of_aggr _ _ _ |- _ =>
+            inversion H; subst
+        end.
+
+      Section WithTags.
+        Context (id_tag aux_tag idx_tag: string).
+
+        Definition aux_ty_for_idx (aux_ty : type -> type) : Prop :=
+          forall t,
+            match aux_ty t with
+            | TRecord tl =>
+                access_record tl id_tag = Success t /\
+                  match access_record tl aux_tag with
+                  | Success (TRecord aux_tl) => access_record aux_tl idx_tag = Success (idx_ty t)
+                  | _ => False
+                  end
+            | _ => False
+            end.
+
+        Definition aux_wf_for_idx (v : value) : Prop :=
+          match v with
+          | VRecord rv =>
+              match access_record rv id_tag with
+              | Success v_id =>
+                  match access_record rv aux_tag with
+                  | Success (VRecord rv_aux) =>
+                      match access_record rv_aux idx_tag with
+                      | Success v_idx =>
+                          idx_wf v_id v_idx
+                      | _ => False
+                      end
+                  | _ => False
+                  end
+              | _ => False
+              end
+          | _ => False
+          end.
+
+        Section sum_to_agg_lookup.
+          Context (tbl : string).
+
+          Definition sum_to_agg_lookup_head (e : expr) :=
+            match e with
+            | EACFold AGSum (EProj LikeBag (EBagOf (EAccess (ELoc tbl0) id_tag0)) x0 (EAccess (EVar x1) attr0)) =>
+                if all_eqb [(tbl, [tbl0]); (attr, [attr0]); (x0, [x1]); (id_tag, [id_tag0]); (x0, [x1])]
+                then EAccess (EAccess (ELoc tbl) aux_tag) idx_tag
+                else e
+            | _ => e
+            end.
+
+          Lemma sum_to_agg_lookup_head_preserve_ty : forall tl t aux_tl (Gstore : tenv),
+              type_wf t -> is_tbl_ty t = true ->
+              map.get Gstore tbl = Some (TRecord tl) ->
+              access_record tl id_tag = Success t ->
+              access_record tl aux_tag = Success (TRecord aux_tl) ->
+              access_record aux_tl idx_tag = Success (idx_ty t) ->
+              preserve_ty Gstore (sum_to_agg_lookup_head).
+          Proof.
+            clear H_NoDup.
+            unfold preserve_ty, is_tbl_ty. intros.
+            repeat destruct_match_hyp; try congruence.
+            repeat destruct_subexpr. simpl.
+            case_match; auto. repeat rewrite Bool.andb_true_r in *.
+            repeat rewrite Bool.andb_true_iff in *; intuition idtac. rewrite eqb_eq in *; subst.
+            repeat invert_type_of_clear. repeat invert_type_of_op_clear. repeat rewrite_map_get_put_hyp.
+            invert_type_of_aggr_clear.
+            repeat (clear_refl; repeat do_injection2).
+            repeat (rewrite_l_to_r; do_injection2).
+            repeat (econstructor; eauto).
+          Qed.
+
+          Lemma sum_to_agg_lookup_head_preserve_sem : forall (Gstore : tenv) (store : locals) tl t aux_tl,
+              type_wf t -> is_tbl_ty t = true ->
+              map.get Gstore tbl = Some (TRecord tl) ->
+              access_record tl id_tag = Success t ->
+              access_record tl aux_tag = Success (TRecord aux_tl) ->
+              access_record aux_tl idx_tag = Success (idx_ty t) ->
+              match map.get store tbl with
+              | Some v => aux_wf_for_idx v
+              | _ => False
+              end ->
+              preserve_sem Gstore store sum_to_agg_lookup_head.
+          Proof.
+            unfold preserve_sem, aux_wf_for_idx; intros.
+            unfold is_tbl_ty, idx_ty in *.
+            apply_locals_wf store.
+            repeat (destruct_match_hyp; try discriminate; intuition idtac; []).
+            invert_type_of_value_clear.
+            pose proof (Forall2_access_record _ _ _ _ _ _ _ _ H16 E1 H2); auto.
+            pose proof (Forall2_access_record _ _ _ _ _ _ _ _ H16 E2 H3); auto.
+            repeat invert_type_of_value_clear.
+            pose proof (Forall2_access_record _ _ _ _ _ _ _ _ H20 E4 H4); auto.
+            repeat destruct_subexpr. unfold sum_to_agg_lookup_head.
+            simpl; case_match; auto.
+            repeat rewrite Bool.andb_true_iff in *; intuition idtac.
+            rewrite eqb_eq in *; subst. repeat clear_refl.
+            unfold idx_wf in *.
+            repeat rewrite_l_to_r.
+            cbn. unfold get_local. rewrite_l_to_r. unfold record_proj.
+            repeat rewrite_l_to_r. unfold to_idx.
+            cbn. unfold get_local. unfold record_proj.
+            rewrite_map_get_put_goal.
+            do 3 f_equal. erewrite map_ext_in; eauto.
+            intros. repeat rewrite_map_get_put_goal. reflexivity.
+          Qed.
+        End sum_to_agg_lookup.
+
+        Section cons_to_add.
+          Definition cons_to_add_head (e : expr) :=
+            match e with
+            | EACFold AGSum (EProj LikeBag (EBagOf (EBinop OCons e1 e2)) x0 e3) =>
+                EBinop OPlus (ELet e1 x0 e3) (EACFold AGSum (EProj LikeBag (EBagOf e2) x0 e3))
+            | _ => e
+            end.
+
+          Lemma cons_to_add_head_preserve_ty : forall (Gstore : tenv),
+              preserve_ty Gstore cons_to_add_head.
+          Proof.
+            unfold preserve_ty; intros. repeat destruct_subexpr.
+            cbn. repeat (case_match; auto).
+            repeat invert_type_of_clear.
+            repeat invert_type_of_op_clear.
+            invert_type_of_aggr_clear.
+            repeat (econstructor; eauto);
+              repeat rewrite_map_get_put_goal; auto;
+              try use_is_NoDup.
+            all: repeat eapply not_free_immut_put_ty2; eauto.
+          Qed.
+
+          Ltac apply_int_binop_Z_add_AC :=
+             intros; unfold apply_int_binop;
+             repeat case_match; auto;
+             rewrite !Z.add_assoc;
+             lazymatch goal with
+               |- context[(?z + _ + _)%Z] =>
+                 rewrite (Z.add_comm z)
+             end; reflexivity.
+
+          Lemma cons_to_add_head_preserve_sem : forall (Gstore : tenv) (store : locals),
+              preserve_sem Gstore store cons_to_add_head.
+          Proof.
+            unfold preserve_sem; intros. repeat destruct_subexpr.
+            cbn [cons_to_add_head]. repeat (case_match; auto; []).
+            cbn in * |-.
+            repeat invert_type_of_clear.
+            repeat invert_type_of_op_clear.
+            cbn.
+            apply_type_sound e1_2.
+            invert_type_of_value_clear.
+            erewrite List.fold_right_change_order;
+            [
+            | apply_int_binop_Z_add_AC
+            | apply list_to_bag_to_list_Permutation ].
+            let pat := open_constr:(bag_to_list (list_to_bag _)) in
+            erewrite List.fold_right_change_order with (l1:=pat);
+            [
+            | apply_int_binop_Z_add_AC | ].
+            2:{ eapply perm_trans.
+                1: apply list_to_bag_to_list_Permutation.
+                eapply Permutation_map, list_to_bag_to_list_Permutation. }
+            cbn.
+            f_equal.
+            erewrite List.fold_right_change_order;
+            [
+            | apply_int_binop_Z_add_AC
+            | eapply Permutation_map, list_to_bag_to_list_Permutation ].
+            reflexivity.
+          Qed.
+        End cons_to_add.
+
+        Ltac invert_tenv_wf_with_globals :=
+          lazymatch goal with H: tenv_wf_with_globals _ _ _ |- _ => inversion H; subst end.
+
+        Lemma sum_to_agg_lookup_head_sound : forall is_tbl_ty' aux_ty aux_wf,
+            aux_ty_for_idx aux_ty ->
+            (forall t, is_tbl_ty' t = true -> is_tbl_ty t = true) ->
+            (forall (v : value), aux_wf v -> aux_wf_for_idx v) ->
+            expr_aug_transf_sound is_tbl_ty' aux_ty aux_wf sum_to_agg_lookup_head.
+        Proof.
+          unfold aux_ty_for_idx, expr_aug_transf_sound; intros.
+          invert_tenv_wf_with_globals.
+          specialize (H tbl_ty). repeat destruct_match_hyp; intuition idtac.
+          1: eapply sum_to_agg_lookup_head_preserve_ty; eauto.
+          1: eapply sum_to_agg_lookup_head_preserve_sem; eauto.
+          lazymatch goal with
+            H: locals_wf ?G ?str, H': map.get ?G _ = _ |- _ =>
+              apply H in H'
+          end.
+          destruct_match_hyp; intuition idtac.
+          lazymatch goal with
+            H: holds_for_all_entries _ ?str, H': map.get ?str _ = _ |- _ =>
+              apply H in H'
+          end.
+          unfold value_wf_with_globals in *. invert_Forall; intuition auto.
+        Qed.
+
+          Lemma cons_to_add_head_sound :
+            expr_transf_sound (locals:=locals) cons_to_add_head.
+          Proof.
+            unfold expr_transf_sound; intros.
+            intuition idtac.
+            1: eapply cons_to_add_head_preserve_ty; eauto.
+            1: eapply cons_to_add_head_preserve_sem; [ | | eauto .. ]; auto.
+          Qed.
+      End WithTags.
+    End WithMap.
+  End WithVars.
+End WithHole.
